src/Analysis/Instances/Interval/Interval_Transfer.thy
@@ -54,7 +54,7 @@ definition enter_ivl ::
 
 lemma enter_frame_ivl_sound:
   assumes gs: "s \<in> \<lbrakk>\<sigma>\<rbrakk>"
-  shows "enter_state s \<in> \<lbrakk>enter_frame_ivl \<sigma>\<rbrakk>"
+  shows "enter_state is_global s \<in> \<lbrakk>enter_frame_ivl \<sigma>\<rbrakk>"
   unfolding enter_frame_ivl_def
 proof (rule enter_frame_D_sound[OF gs])
   show "gamma ivl_top = UNIV" by (simp add: gamma_ivl_top)
@@ -62,7 +62,7 @@ qed
 
 lemma enter_ivl_sound:
   assumes gs: "s \<in> \<lbrakk>\<sigma>\<rbrakk>"
-  shows "bind_formals xs (map (\<lambda>e. aval e s) es) (enter_state s)
+  shows "bind_formals xs (map (\<lambda>e. aval e s) es) (enter_state is_global s)
            \<in> \<lbrakk>enter_ivl xs es \<sigma>\<rbrakk>"
   unfolding enter_ivl_def
 proof (rule enter_D_sound[OF gs])
@@ -96,7 +96,7 @@ lemma ivl_tf_sound_assume_not:
 
 lemma ivl_tf_sound_enter:
   "\<forall>xs (es::aexp list) \<sigma>. \<forall>st \<in> \<lbrakk>\<sigma>\<rbrakk>.
-     bind_formals xs (map (\<lambda>e. aval e st) es) (enter_state st)
+     bind_formals xs (map (\<lambda>e. aval e st) es) (enter_state is_global st)
        \<in> \<lbrakk>tf_enter ivl_tf xs es \<sigma>\<rbrakk>"
   unfolding ivl_tf_def by (simp add: enter_ivl_sound)
 
@@ -109,7 +109,8 @@ proof (rule sound_transferI)
   show "\<And>b \<sigma> s. s \<in> \<lbrakk>\<sigma>\<rbrakk> \<Longrightarrow> \<not> bval b s \<Longrightarrow> s \<in> \<lbrakk>tf_assume_not ivl_tf b \<sigma>\<rbrakk>"
     using ivl_tf_sound_assume_not by blast
   show "\<And>xs es \<sigma> s. s \<in> \<lbrakk>\<sigma>\<rbrakk> \<Longrightarrow>
-     bind_formals xs (map (\<lambda>e. aval e s) es) (enter_state s) \<in> \<lbrakk>tf_enter ivl_tf xs es \<sigma>\<rbrakk>"
+     bind_formals xs (map (\<lambda>e. aval e s) es) (enter_state is_global s)
+       \<in> \<lbrakk>tf_enter ivl_tf xs es \<sigma>\<rbrakk>"
     using ivl_tf_sound_enter by blast
   show "tf_combine ivl_tf = combine_abs"
     unfolding ivl_tf_def by simp
